src/HOL/Matrix/cplex/Cplex.thy
@@ -19,7 +19,7 @@ lemma spm_mult_le_dual_prts:
   "sorted_sparse_matrix r1"
   "sorted_sparse_matrix r2"
   "sorted_spvec b"
-  "le_spmat ([], y)"
+  "le_spmat [] y"
   "sparse_row_matrix A1 \<le> A"
   "A \<le> sparse_row_matrix A2"
   "sparse_row_matrix c1 \<le> c"
@@ -28,10 +28,10 @@ lemma spm_mult_le_dual_prts:
   "x \<le> sparse_row_matrix r2"
   "A * x \<le> sparse_row_matrix (b::('a::lordered_ring) spmat)"
   shows
-  "c * x \<le> sparse_row_matrix (add_spmat (mult_spmat y b,
+  "c * x \<le> sparse_row_matrix (add_spmat (mult_spmat y b)
   (let s1 = diff_spmat c1 (mult_spmat y A2); s2 = diff_spmat c2 (mult_spmat y A1) in 
-  add_spmat (mult_spmat (pprt_spmat s2) (pprt_spmat r2), add_spmat (mult_spmat (pprt_spmat s1) (nprt_spmat r2), 
-  add_spmat (mult_spmat (nprt_spmat s2) (pprt_spmat r1), mult_spmat (nprt_spmat s1) (nprt_spmat r1)))))))"
+  add_spmat (mult_spmat (pprt_spmat s2) (pprt_spmat r2)) (add_spmat (mult_spmat (pprt_spmat s1) (nprt_spmat r2)) 
+  (add_spmat (mult_spmat (nprt_spmat s2) (pprt_spmat r1)) (mult_spmat (nprt_spmat s1) (nprt_spmat r1))))))"
   apply (simp add: Let_def)
   apply (insert assms)
   apply (simp add: sparse_row_matrix_op_simps algebra_simps)  
@@ -49,7 +49,7 @@ lemma spm_mult_le_dual_prts_no_let:
   "sorted_sparse_matrix r1"
   "sorted_sparse_matrix r2"
   "sorted_spvec b"
-  "le_spmat ([], y)"
+  "le_spmat [] y"
   "sparse_row_matrix A1 \<le> A"
   "A \<le> sparse_row_matrix A2"
   "sparse_row_matrix c1 \<le> c"
@@ -58,8 +58,8 @@ lemma spm_mult_le_dual_prts_no_let:
   "x \<le> sparse_row_matrix r2"
   "A * x \<le> sparse_row_matrix (b::('a::lordered_ring) spmat)"
   shows
-  "c * x \<le> sparse_row_matrix (add_spmat (mult_spmat y b,
-  mult_est_spmat r1 r2 (diff_spmat c1 (mult_spmat y A2)) (diff_spmat c2 (mult_spmat y A1))))"
+  "c * x \<le> sparse_row_matrix (add_spmat (mult_spmat y b)
+  (mult_est_spmat r1 r2 (diff_spmat c1 (mult_spmat y A2)) (diff_spmat c2 (mult_spmat y A1))))"
   by (simp add: assms mult_est_spmat_def spm_mult_le_dual_prts[where A=A, simplified Let_def])
 
 use "matrixlp.ML"
